WIP

src/Renaming.v
@@ -1,27 +1,195 @@
 Require Import Label PeanoNat Psatz Ring Compare_dec StrictProp.
-Require Import Var VarEquations.
+Require Import Var VarEquations RawRenaming.
+
+Fixpoint apply_raw_renaming_unmatched_var r v {struct r} :=
+  match r with
+  | raw_renaming_id => v
+  | raw_renaming_extend vl r vr =>
+    shift_var
+      vl (apply_raw_renaming_unmatched_var r (unshift_var vr v))
+  end.
+
+Definition is_normal_raw_renaming_extension vl r vr :=
+  negb (is_shifting_var
+          vl (apply_raw_renaming_unmatched_var r vr)).
+
+Fixpoint is_all_normal_raw_renaming r :=
+  match r with
+  | raw_renaming_id => true
+  | raw_renaming_extend vl r' vr =>
+    andb
+      (is_normal_raw_renaming_extension vl r' vr)
+      (is_all_normal_raw_renaming r')
+  end.
+
+Definition is_less_equal_raw_renaming_var v r :=
+  match r with
+  | raw_renaming_id => true
+  | raw_renaming_extend _ _ v' => is_less_equal_var v v'
+  end.
+
+Fixpoint is_all_ordered_raw_renaming r :=
+  match r with
+  | raw_renaming_id => true
+  | raw_renaming_extend vl r' vr =>
+    andb
+      (is_less_equal_raw_renaming_var vr r')
+      (is_all_ordered_raw_renaming r')
+  end.
+
+Definition is_normalized_raw_renaming r :=
+  andb
+    (is_all_normal_raw_renaming r)
+    (is_all_ordered_raw_renaming r).
+
+Lemma is_normalized_raw_renaming_extend vl r vr :
+  is_normalized_raw_renaming (raw_renaming_extend vl r vr)
+  = andb
+      (is_normalized_raw_renaming r)
+      (andb
+         (is_normal_raw_renaming_extension vl r vr)
+         (is_less_equal_raw_renaming_var vr r)).
+Proof.
+  unfold is_normalized_raw_renaming; cbn; ring.
+  (* TODO: maybe btauto insteead of ring? *)
+Qed.
+
+Lemma is_normalized_raw_renaming_from_extend vl r vr :
+  is_normalized_raw_renaming (raw_renaming_extend vl r vr) = true ->
+  is_normalized_raw_renaming r = true.
+Proof.
+  rewrite is_normalized_raw_renaming_extend.
+  rewrite! Bool.andb_true_iff.
+  easy.
+Qed.
+
+Lemma apply_normal_raw_renaming_unmatched_var r v :
+  is_all_normal_raw_renaming r = true ->
+  (apply_raw_renaming_unmatched_var r v
+   = apply_raw_renaming_var r v)
+  \/ ((apply_raw_renaming_unmatched_var r v
+       = apply_raw_renaming_unmatched_var r (succ_var v))
+      /\ (is_shifting_var
+            (apply_raw_renaming_var r v)
+            (apply_raw_renaming_unmatched_var r v)
+          = false)).
+Proof.
+  generalize dependent v.
+  induction r as [|vl r IHr vr]; cbn; intros v Heq.
+  - left; easy.
+  - rewrite Bool.andb_true_iff in Heq; destruct Heq as [Heq1 Heq2].
+    case_vars_eq v vr.
+    + right; split; try easy; subst.
+      unfold is_normal_raw_renaming_extension in Heq1.
+      rewrite Bool.negb_true_iff in Heq1.
+      rewrite is_shifting_false_shift; easy.
+    + destruct (IHr (unshift_var vr v) Heq2)
+        as [Heq3|[Heq3 Heq4]]; [left|right;split].
+      * rewrite Heq3; easy.
+      * rewrite Heq3.
+        rewrite succ_var_unshift_var_neq by congruence.
+        easy.
+      * rewrite <- transposed_is_shifting_var.
+        rewrite reducible_transposed_2
+          with (v1 := apply_raw_renaming_var
+                        r (unshift_var vr v)) by easy.
+        easy.
+Qed.
+
+Definition is_less_than_raw_renaming_var v r :=
+  match r with
+  | raw_renaming_id => true
+  | raw_renaming_extend _ _ v' => is_less_than_var v v'
+  end.
+
+Lemma is_less_than_raw_renaming_var_extend v v' r :
+  is_less_equal_raw_renaming_var v' r = true ->
+  is_less_than_var v v' = true ->
+  is_less_than_raw_renaming_var v r = true.
+Proof.
+  intros Heq1 Heq2.
+  destruct r as [|vl' r vr']; cbn in *;try easy.
+  apply is_less_than_less_equal_var_transitive with v'; easy.
+Qed.
+
+Lemma apply_normalized_raw_renaming_unmatched_var r v :
+  is_all_ordered_raw_renaming r = true ->
+  is_less_than_raw_renaming_var v r = true ->
+  apply_raw_renaming_var r v
+  = apply_raw_renaming_unmatched_var r v.
+Proof.
+  intros Heq1 Heq2.
+  induction r as [|vl' r IHr vr']; cbn in *; try easy.
+  rewrite Bool.andb_true_iff in Heq1; destruct Heq1.
+  case_vars vr' v; rewrite IHr; try easy;
+    apply is_less_than_raw_renaming_var_extend with vr';
+      reduce_vars; easy.
+Qed.
+
+Lemma is_normalized_equivalence r1 r2 :
+  is_normalized_raw_renaming r1 = true ->
+  is_normalized_raw_renaming r2 = true ->
+  apply_raw_renaming_var r1
+  =v= apply_raw_renaming_var r2 ->
+  r1 = r2.
+Proof.
+  generalize dependent r2.
+  induction r1 as [|vl1 r1 IHr vr1]; intros r2 Heq1 Heq2 Heq3;
+    destruct r2 as [|vl2 r2 vr2]; try easy.
+  - specialize (Heq3 (succ_var vr2)) as Heq4.
+    rewrite apply_normalized_raw_renaming_unmatched_var
+      with (r := raw_renaming_extend _ _ _) in Heq4.
+    + admit.
+    + unfold is_normalized_raw_renaming in Heq2;
+        rewrite Bool.andb_true_iff in Heq2; destruct Heq2; easy.
+    + cbn. reduce_vars.
+
+specialize (Heq3 vr2) as Heq4;
+      reduce_vars; rewrite Heq4 in *.
+    
+    admit.
+  - specialize (Heq3 vr1) as Heq4;
+      reduce_vars; rewrite Heq4 in *.
+    
 
 Fixpoint is_interesting_raw_renaming_extension vl r vr :=
   match r with
   | raw_renaming_id => negb (var_eqb vl vr)
   | raw_renaming_extend vl' r vr' =>
-    is_interesting_raw_renaming_extension
-      (unshift_var vl' vl) r (unshift_var vr' vr)
+      is_interesting_raw_renaming_extension
+         (unshift_var vl' vl) r (unshift_var vr' vr)
   end.
 
-Fixpoint is_all_interesting_raw_renaming r :=
+Fixpoint is_needed_raw_renaming_extension vl r :=
+  match r with
+  | raw_renaming_id => false
+  | raw_renaming_extend vl' r vr' =>
+    (orb
+       (is_shifting_var vl vl')
+       (is_needed_raw_renaming_extension (unshift_var vl' vl) r))
+  end.
+
+Definition is_needed_or_interesting_raw_renaming_extension
+           vl r vr :=
+  (orb
+     (is_needed_raw_renaming_extension vl r)
+     (is_interesting_raw_renaming_extension vl r vr)).
+Arguments is_needed_or_interesting_raw_renaming_extension vl r vr /.
+
+Fixpoint is_all_needed_or_interesting_raw_renaming r :=
   match r with
   | raw_renaming_id => true
   | raw_renaming_extend vl r' vr =>
     andb
-      (is_interesting_raw_renaming_extension vl r' vr)
-      (is_all_interesting_raw_renaming r')
+      (is_needed_or_interesting_raw_renaming_extension vl r' vr)
+      (is_all_needed_or_interesting_raw_renaming r')
   end.
 
-Lemma is_all_interesting_raw_renaming_from_extend {vl r vr} :
-  is_all_interesting_raw_renaming
+Lemma is_all_needed_or_interesting_raw_renaming_from_extend
+      {vl r vr} :
+  is_all_needed_or_interesting_raw_renaming
     (raw_renaming_extend vl r vr) = true ->
-  is_all_interesting_raw_renaming r = true.
+  is_all_needed_or_interesting_raw_renaming r = true.
 Proof.
   destruct r; cbn;
     try rewrite Bool.andb_true_iff; easy.
@@ -33,83 +201,37 @@ Fixpoint raw_renaming_extend_boring vl r vr :=
       if (var_eqb vl vr) then Some r
       else None
   | raw_renaming_extend vl' r vr' =>
-    match raw_renaming_extend_boring
+    match is_shifting_var vl vl' with
+    | true => None
+    | false =>
+      match raw_renaming_extend_boring
               (unshift_var vl' vl) r (unshift_var vr' vr)
-    with
-    | None => None
-    | Some r =>
-      Some (raw_renaming_extend
-              (shift_var vl vl') r (shift_var vr vr'))
+      with
+      | None => None
+      | Some r =>
+        Some (raw_renaming_extend
+                (shift_var vl vl') r (shift_var vr vr'))
+      end
     end
   end.
 
-Lemma is_interesting_raw_renaming_extend_boring_none vl r vr :
+Lemma is_needed_or_interesting_raw_renaming_extend_boring_none
+      vl r vr :
   raw_renaming_extend_boring vl r vr = None ->
-  is_interesting_raw_renaming_extension vl r vr = true.
+  is_needed_or_interesting_raw_renaming_extension vl r vr = true.
 Proof.
   generalize dependent vl.
   generalize dependent vr.
   induction r as [|vl' r IHr vr']; cbn; intros vr vl Heq.
-  - destruct (var_eqb vl vr); easy.
-  - apply IHr.
+  - destruct var_eqb; easy.
+  - destruct is_shifting_var; try easy.
+    apply IHr.
     destruct (raw_renaming_extend_boring
                 (unshift_var vl' vl) r (unshift_var vr' vr));
       easy.
 Qed.
 
-(* TODO move to VarEquations.v *)
-Lemma succ_var_injective v1 v2 :
-  v1 <> v2 ->
-  succ_var v1 <> succ_var v2.
-Proof.
-  intros Hneq Heq; apply Hneq.
-  replace v1 with (pred_var (succ_var v1))
-    by (reduce_vars; easy).
-  replace v2 with (pred_var (succ_var v2))
-    by (reduce_vars; easy).
-  congruence.
-Qed.
-
-Lemma mk_var_label_injective v1 v2 :
-  v_label_opt v1 <> v_label_opt v2 ->
-  v1 <> v2.
-Proof.
-  intros Hneq Heq; apply Hneq.
-  rewrite Heq; easy.
-Qed.
-
-Lemma var_eqb_false v1 v2 :
-  (var_eqb v1 v2 = false) <-> v1 <> v2.
-Proof.
-  unfold var_eqb.
-  destruct (var_dec v1 v2); easy.
-Qed.
-
-Lemma var_eqb_true v1 v2 :
-  (var_eqb v1 v2 = true) <-> v1 = v2.
-Proof.
-  unfold var_eqb.
-  destruct (var_dec v1 v2); easy.
-Qed.
-
-Lemma shift_neq vl1 vl2 vr1 vr2 :
-  vl1 <> vr1 ->
-  unshift_var vl1 vl2 = unshift_var vr1 vr2 ->
-  shift_var vl2 vl1 <> shift_var vr2 vr1.
-Proof.
-  intros Hneq Heq.
-  destruct (label_opt_dec (v_label_opt vl1) (v_label_opt vr1)).
-  - case_vars vl1 vl2; case_vars vr1 vr2; subst;
-      autorewrite with reduce_vars_beta in *;
-      try easy; try congruence;
-        solve [rewrite red_var_neq
-                by solve_v_label_opt_equation;
-               reduce_vars_beta; lia].
-  - apply mk_var_label_injective; reduce_vars_beta; easy.
-Qed.
-
-Lemma is_interesting_raw_renaming_extend_boring_some_ind
-      r1 :
+Lemma is_interesting_raw_renaming_extend_boring_some_ind r1 :
   forall r2 vl1 vl2 vr1 vr2,
   is_interesting_raw_renaming_extension vl1 r1 vr1 = true ->
   raw_renaming_extend_boring
@@ -117,14 +239,16 @@ Lemma is_interesting_raw_renaming_extend_boring_some_ind
   is_interesting_raw_renaming_extension
     (shift_var vl2 vl1) r2 (shift_var vr2 vr1) = true.
 Proof.
-  induction r1 as [|vl5 r1 IHr1 vr5]; cbn; intros * Heq1 Heq2.
-  - destruct
-      (var_eqb (unshift_var vl1 vl2) (unshift_var vr1 vr2))
-      eqn:Heq3; try easy.
+  induction r1 as [|vl3 r1 IHr1 vr3]; cbn; intros * Heq1 Heq2.
+  - case_vars_eq vl1 vr1.
+    case_vars_eq
+      (unshift_var vl1 vl2) (unshift_var vr1 vr2).
     injection Heq2 as <-; cbn.
-    rewrite Bool.negb_true_iff, var_eqb_false, var_eqb_true in *.
-    apply shift_neq; easy.
-  - destruct raw_renaming_extend_boring eqn:Heq3; try easy.
+    apply Bool.negb_true_iff, var_eqb_false.
+    apply transpose_irreducible_pop_push_nested; try easy.
+  - destruct (is_shifting_var (unshift_var vl1 vl2) vl3) eqn:Heq3;
+      try easy.
+    destruct raw_renaming_extend_boring eqn:Heq4; try easy.
     injection Heq2 as <-; cbn.
     rewrite <- transpose_pops_reverse_middle.
     rewrite transpose_pushes_reverse_middle.
@@ -134,10 +258,34 @@ Proof.
     easy.
 Qed.
 
-Lemma is_interesting_raw_renaming_extend_boring_some vl r1 vr r2 :
-  is_all_interesting_raw_renaming r1 = true ->
+Lemma is_needed_raw_renaming_extend_boring_some_ind r1 :
+  forall r2 vl1 vl2 vr,
+  is_needed_raw_renaming_extension vl1 r1 = true ->
+  raw_renaming_extend_boring
+    (unshift_var vl1 vl2) r1 vr = Some r2 ->
+  is_needed_raw_renaming_extension (shift_var vl2 vl1) r2 = true.
+Proof.
+  induction r1 as [|vl3 r1 IHr1 vr3];
+    cbn; intros * Heq1 Heq2; try easy.
+  destruct (is_shifting_var (unshift_var vl1 vl2) vl3) eqn:Heq3;
+    try easy.
+  destruct raw_renaming_extend_boring eqn:Heq4; try easy.
+  injection Heq2 as <-; cbn.
+  rewrite Bool.orb_true_iff in *.
+  destruct Heq1 as [Heq1|Heq1]; [left|right].
+  - rewrite <- transposed_is_shifting_var.
+    rewrite transpose_pushes_squared_left; easy.
+  - rewrite <- transpose_pops_reverse_middle.
+    apply IHr1 with (vr := unshift_var vr3 vr); try easy.
+    rewrite transpose_pops_reverse_right.
+    easy.
+Qed.
+
+Lemma is_needed_or_interesting_raw_renaming_extend_boring_some
+      vl r1 vr r2 :
+  is_all_needed_or_interesting_raw_renaming r1 = true ->
   raw_renaming_extend_boring vl r1 vr = Some r2 ->
-  is_all_interesting_raw_renaming r2 = true.
+  is_all_needed_or_interesting_raw_renaming r2 = true.
 Proof.
   generalize dependent vl.
   generalize dependent vr.
@@ -146,12 +294,16 @@ Proof.
     intros r2 vr vl Heq1 Heq2.
   - destruct var_eqb; try easy.
     injection Heq2 as <-; easy.
-  - rewrite Bool.andb_true_iff in Heq1;
-      destruct Heq1 as [Heq1 Heq3].
-    destruct raw_renaming_extend_boring eqn:Heq4; try easy.
+  - destruct is_shifting_var; try easy.
+    destruct raw_renaming_extend_boring eqn:Heq3; try easy.
     injection Heq2 as <-; cbn.
-    rewrite Bool.andb_true_iff; split.
-    + apply is_interesting_raw_renaming_extend_boring_some_ind
+    rewrite! Bool.andb_true_iff, Bool.orb_true_iff in *.
+    destruct Heq1 as [Heq1 Heq4]; split; [destruct Heq1|].
+    + left.
+      apply is_needed_raw_renaming_extend_boring_some_ind
+        with (r1 := r1) (vr := unshift_var vr2 vr); easy.
+    + right.
+      apply is_interesting_raw_renaming_extend_boring_some_ind
         with (r1 := r1); easy.
     + apply IHr1
         with (vl := unshift_var vl2 vl) (vr := unshift_var vr2 vr);
@@ -164,17 +316,18 @@ Definition interesting_raw_renaming_extend vl r vr :=
   | None => raw_renaming_extend vl r vr
   end.
 
-Lemma is_all_interesting_raw_renaming_extend vl r vr :
-  is_all_interesting_raw_renaming r = true ->
-  is_all_interesting_raw_renaming
+Lemma is_all_needed_or_interesting_raw_renaming_extend vl r vr :
+  is_all_needed_or_interesting_raw_renaming r = true ->
+  is_all_needed_or_interesting_raw_renaming
     (interesting_raw_renaming_extend vl r vr) = true.
 Proof.
   intro Heq1; unfold interesting_raw_renaming_extend.
   destruct (raw_renaming_extend_boring vl r vr) eqn:Heq2; cbn.
-  - apply is_interesting_raw_renaming_extend_boring_some
+  - apply is_needed_or_interesting_raw_renaming_extend_boring_some
       in Heq2; easy.
   - rewrite Bool.andb_true_iff; split; try easy.
-    apply is_interesting_raw_renaming_extend_boring_none; easy.
+    apply is_needed_or_interesting_raw_renaming_extend_boring_none;
+      easy.
 Qed.
 
 Lemma is_interesting_interesting_raw_renaming_extend_ind r1 :
@@ -185,15 +338,16 @@ Lemma is_interesting_interesting_raw_renaming_extend_ind r1 :
     is_interesting_raw_renaming_extension vl2 r2 vr2 = true.
 Proof.
   induction r1 as [|vl3 r1 IHr1 vr3]; cbn; intros * Heq1 Heq2.
-  - destruct (var_eqb vl1 vr1) eqn:Heq3; try easy.
+  - case_vars_eq vl1 vr1.
     injection Heq1 as <-; cbn.
-    rewrite Bool.negb_true_iff, var_eqb_false, var_eqb_true in *.
-    intros Heq4; subst; easy.
-  - destruct raw_renaming_extend_boring eqn:Heq3; try easy.
+    case_vars_eq (unshift_var vl1 vl2) (unshift_var vr1 vr2);
+      easy.
+  - destruct (is_shifting_var vl1 vl3); try easy.
+    destruct raw_renaming_extend_boring eqn:Heq4; try easy.
     injection Heq1 as <-; cbn.
-    eapply IHr1 with (vl2 := unshift_var (shift_var vl1 vl3) vl2)
-      (vr2 := unshift_var (shift_var vr1 vr3) vr2)
-      in Heq3; try easy.
+    apply IHr1 with (vl2 := unshift_var (shift_var vl1 vl3) vl2)
+        (vr2 := unshift_var (shift_var vr1 vr3) vr2)
+        in Heq4; try easy.
     rewrite transpose_pops_reverse_right.
     rewrite transpose_pushes_reverse_left.
     easy.
@@ -213,21 +367,6 @@ Proof.
     with (r1 := r) (vl1 := vl1) (vr1 := vr1); easy.
 Qed.
 
-Definition is_ordered_raw_renaming_var v r :=
-  match r with
-  | raw_renaming_id => true
-  | raw_renaming_extend v' _ _ => is_less_equal_vars v v'
-  end.
-
-Fixpoint is_all_ordered_raw_renaming r :=
-  match r with
-  | raw_renaming_id => true
-  | raw_renaming_extend vl r' vr =>
-    andb
-      (is_ordered_raw_renaming_var vl r')
-      (is_all_ordered_raw_renaming r')
-  end.
-
 Lemma is_all_ordered_raw_renaming_from_extend {vl r vr} :
   is_all_ordered_raw_renaming
     (raw_renaming_extend vl r vr) = true ->
@@ -239,17 +378,17 @@ Qed.
 
 (* TODO : move to var equations *)
 Lemma succ_var_monotonic v1 v2 :
-  is_less_equal_vars (succ_var v1) (succ_var v2)
-  = is_less_equal_vars v1 v2.
+  is_shifting_var (succ_var v1) (succ_var v2)
+  = is_shifting_var v1 v2.
 Proof.
   case_vars v1 v2; easy.
 Qed.
 
 (* TODO : move to var equations *)
 Lemma is_less_equal_shift v1 v2 v3 :
-  is_less_equal_vars
+  is_less_equal_var
     (shift_var v3 v1) (shift_var (unshift_var v1 v3) v2)
-  = is_less_equal_vars v1 v2.
+  = is_less_equal_var v1 v2.
 Proof.
   case_vars v1 v3;
     case_vars (unshift_var v1 v3) v2; try easy.
@@ -258,24 +397,25 @@ Qed.
 
 Lemma is_ordered_raw_renaming_less_equal_var v1 v2 r :
   is_ordered_raw_renaming_var v1 r = true ->
-  is_less_equal_vars v2 v1 = true ->
+  is_less_equal_var v2 v1 = true ->
   is_ordered_raw_renaming_var v2 r = true.
 Proof.
   destruct r; cbn; intros Heq1 Heq2; try easy.
-  apply is_less_equal_vars_transitive with (v2 := v1); easy.
+  apply is_less_equal_var_transitive with (v2 := v1); easy.
 Qed.
 
 Lemma is_ordered_raw_renaming_extend_boring_some_ind r1 :
-  forall vl1 vr1 r2 vl2,
+  forall vl1 vr1 r2 vr2,
     raw_renaming_extend_boring
-      (unshift_var vl1 vl2) r1 vr1 = Some r2 ->
-    is_ordered_raw_renaming_var (shift_var vl2 vl1) r2
-    = is_ordered_raw_renaming_var vl1 r1.
+      vl1 r1 (unshift_var vr1 vr2) = Some r2 ->
+    is_ordered_raw_renaming_var (shift_var vr2 vr1) r2
+    = is_ordered_raw_renaming_var vr1 r1.
 Proof.
   destruct r1 as [|vl3 r3 vr3]; cbn; intros * Heq1.
-  - destruct var_eqb; try easy.
+  - case_vars_eq vl1 (unshift_var vr1 vr2).
     injection Heq1 as <-; easy.
-  - destruct raw_renaming_extend_boring eqn:Heq2; try easy.
+  - destruct is_shifting_var; try easy.
+    destruct raw_renaming_extend_boring eqn:Heq2; try easy.
     injection Heq1 as <-; cbn.
     apply is_less_equal_shift.
 Qed.
@@ -292,12 +432,13 @@ Proof.
     cbn; intros r' vr vl Heq1 Heq2.
   - destruct var_eqb; try easy.
     injection Heq1 as <-; easy.
-  - destruct raw_renaming_extend_boring eqn:Heq3; try easy.
+  - destruct is_shifting_var; try easy.
+    destruct raw_renaming_extend_boring eqn:Heq3; try easy.
     injection Heq1 as <-; cbn.
     rewrite Bool.andb_true_iff in Heq2.
     destruct Heq2 as [Heq2 Heq5].
     rewrite is_ordered_raw_renaming_extend_boring_some_ind
-      with (r1 := r) (vr1 := unshift_var vr' vr); try easy.
+      with (r1 := r) (vl1 := unshift_var vl' vl); try easy.
     rewrite Heq2; cbn.
     apply IHr
       with (vl := unshift_var vl' vl) (vr := unshift_var vr' vr);
@@ -319,27 +460,28 @@ Proof.
 Qed.
 
 Lemma is_ordered_interesting_raw_renaming_extend_ind r1 :
-  forall vl1 vr1 r2 vl2,
+  forall vl1 vr1 r2 vr2,
     raw_renaming_extend_boring vl1 r1 vr1 = Some r2 ->
-    is_less_equal_vars vl2 vl1 = true ->
-    is_ordered_raw_renaming_var vl2 r1 = true ->
-    is_ordered_raw_renaming_var vl2 r2 = true.
+    is_less_equal_var vr2 vr1 = true ->
+    is_ordered_raw_renaming_var vr2 r1 = true ->
+    is_ordered_raw_renaming_var vr2 r2 = true.
 Proof.
   destruct r1 as [|vl3 r vr3]; cbn; intros * Heq1 Heq2 Heq3.
-  - destruct var_eqb; try easy.
+  - case_vars_eq vl1 vr1.
     injection Heq1 as <-; easy.
-  - destruct raw_renaming_extend_boring; try easy.
+  - destruct is_shifting_var; try easy.
+    destruct raw_renaming_extend_boring; try easy.
     injection Heq1 as <-; cbn.
-    apply is_less_equal_vars_transitive with vl3; try easy.
-    apply is_less_equal_vars_shift_r.
+    apply is_less_equal_var_transitive with vr3; try easy.
+    apply is_less_equal_var_shift_r.
 Qed.
 
 Lemma is_ordered_interesting_raw_renaming_extend
-      vl1 r vr1 vl2 :
-  is_less_equal_vars vl2 vl1 = true ->
-  is_ordered_raw_renaming_var vl2 r = true ->
+      vl1 r vr1 vr2 :
+  is_less_equal_var vr2 vr1 = true ->
+  is_ordered_raw_renaming_var vr2 r = true ->
   is_ordered_raw_renaming_var
-    vl2 (interesting_raw_renaming_extend vl1 r vr1) = true.
+    vr2 (interesting_raw_renaming_extend vl1 r vr1) = true.
 Proof.
   unfold interesting_raw_renaming_extend.
   destruct raw_renaming_extend_boring eqn:Heq1;
@@ -348,33 +490,8 @@ Proof.
     with (r1 := r) (vl1 := vl1) (vr1 := vr1); easy.
 Qed.
 
-Definition is_normalized_raw_renaming r :=
-  andb
-    (is_all_interesting_raw_renaming r)
-    (is_all_ordered_raw_renaming r).
-
 Definition normalized_raw_renaming r :=
   if is_normalized_raw_renaming r then sUnit else sEmpty.
-
-Lemma is_normalized_raw_renaming_extend vl r vr :
-  is_normalized_raw_renaming (raw_renaming_extend vl r vr)
-  = andb
-      (is_normalized_raw_renaming r)
-      (andb
-         (is_interesting_raw_renaming_extension vl r vr)
-         (is_ordered_raw_renaming_var vl r)).
-Proof.
-  unfold is_normalized_raw_renaming; cbn; ring.
-Qed.
-
-Lemma is_normalized_raw_renaming_from_extend {vl r vr} :
-  is_normalized_raw_renaming (raw_renaming_extend vl r vr) = true ->
-  is_normalized_raw_renaming r = true.
-Proof.
-  rewrite is_normalized_raw_renaming_extend.
-  rewrite! Bool.andb_true_iff.
-  easy.
-Qed.
 
 Lemma normalized_raw_renaming_from_extend {vl r vr} :
   normalized_raw_renaming (raw_renaming_extend vl r vr) ->
@@ -387,7 +504,7 @@ Qed.
 
 Lemma is_normalized_interesting_raw_renaming_extend vl r vr :
   is_normalized_raw_renaming r = true ->
-  is_ordered_raw_renaming_var vl r = true ->
+  is_ordered_raw_renaming_var vr r = true ->
   is_normalized_raw_renaming
     (interesting_raw_renaming_extend vl r vr) = true.
 Proof.
@@ -395,7 +512,7 @@ Proof.
   rewrite! Bool.andb_true_iff.
   intros [Heq1 Heq2] Heq3.
   split.
-  - apply is_all_interesting_raw_renaming_extend; easy.
+  - apply is_all_needed_or_interesting_raw_renaming_extend; easy.
   - apply is_all_ordered_interesting_raw_renaming_extend; cbn.
     rewrite! Bool.andb_true_iff; easy.
 Qed.
@@ -404,7 +521,7 @@ Fixpoint normalized_raw_renaming_extend vl r vr :=
   match r with
   | raw_renaming_id => interesting_raw_renaming_extend vl r vr
   | raw_renaming_extend vl' r' vr' =>
-    if is_less_equal_vars vl vl' then
+    if is_less_equal_var vr vr' then
       interesting_raw_renaming_extend vl r vr
     else
       raw_renaming_extend
@@ -427,30 +544,34 @@ Proof.
   generalize dependent vl1.
   induction r1 as [|vl3 r2 IHr vr3]; cbn; intros * Heq1.
   - apply is_interesting_interesting_raw_renaming_extend; easy.
-  - destruct is_less_equal_vars; cbn.
+  - destruct is_less_equal_var; cbn.
     + apply is_interesting_interesting_raw_renaming_extend; easy.
     + rewrite IHr; cbn; try easy.
       rewrite transpose_pops_reverse_right.
       rewrite transpose_pushes_reverse_left; easy.
 Qed.
 
-Lemma is_all_interesting_normalized_raw_renaming_extend vl r vr :
-  is_all_interesting_raw_renaming r = true ->
-  is_all_interesting_raw_renaming
+Lemma is_all_needed_or_interesting_normalized_raw_renaming_extend
+      vl r vr :
+  is_all_needed_or_interesting_raw_renaming r = true ->
+  is_all_needed_or_interesting_raw_renaming
     (normalized_raw_renaming_extend vl r vr) = true.
 Proof.
   generalize dependent vr.
   generalize dependent vl.
   induction r as [|vl' r IHr vr']; cbn; intros vl vr Heq1.
-  - apply is_all_interesting_raw_renaming_extend; easy.
-  - destruct is_less_equal_vars eqn:Heq3; cbn.
-    + apply is_all_interesting_raw_renaming_extend; easy.
-    + rewrite Bool.andb_true_iff in Heq1.
-      destruct Heq1 as [Heq1 Heq2].
-      rewrite! Bool.andb_true_iff; split; auto.
-      apply is_interesting_normalized_raw_renaming_extend; cbn.
-      rewrite transpose_pops_squared_right.
-      rewrite transpose_pushes_squared_left; easy.
+  - apply is_all_needed_or_interesting_raw_renaming_extend; easy.
+  - destruct is_less_equal_var eqn:Heq3; cbn.
+    + apply is_all_needed_or_interesting_raw_renaming_extend; easy.
+    + rewrite Bool.andb_true_iff, Bool.orb_true_iff in *.
+      destruct Heq1 as [Heq1 Heq2]; split; auto.
+      destruct Heq1.
+      * left.
+        admit.
+      * right.
+        apply is_interesting_normalized_raw_renaming_extend; cbn.
+        rewrite transpose_pops_squared_right.
+        rewrite transpose_pushes_squared_left; easy.
 Qed.
 
 Lemma is_ordered_normalized_raw_renaming_extend vl1 r1 vr1 vl2 :
