src/Var.v
@@ -299,12 +299,31 @@ Definition swap_var : var_op 2 2 :=
     end.
 Arguments swap_var voo : simpl nomatch.
 
+(* [v1] is "shifting" [v2] another if [shift_var v1 v2 <> v2] *)
+
+Definition is_shifting_var v1 v2 :=
+  andb
+    (label_opt_eqb (v_label_opt v1) (v_label_opt v2))
+    (leb (v_nat v1) (v_nat v2)).
+
+Definition shifts_var v1 v2 :=
+  if is_shifting_var v1 v2 then sUnit
+  else sEmpty.
+
 (* Total ordering on vars *)
 
-Definition is_less_equal_vars v1 v2 :=
+Definition is_less_equal_var v1 v2 :=
   orb
     (is_less_than_label_opt (v_label_opt v1) (v_label_opt v2))
-    (andb
-       (label_opt_eqb (v_label_opt v1) (v_label_opt v2))
-       (leb (v_nat v1) (v_nat v2))).
+    (is_shifting_var v1 v2).
 
+Definition less_equal_var v1 v2 :=
+  if is_less_equal_var v1 v2 then sUnit
+  else sEmpty.
+
+Definition is_less_than_var v v' :=
+  negb (is_less_equal_var v' v).
+
+Definition less_than_var v1 v2 :=
+  if is_less_than_var v1 v2 then sUnit
+  else sEmpty.
